Iteration 2... fail

src/automata.v
@@ -2,7 +2,9 @@ Require Import
   Lists.List
   Init.Nat
   Lia
+  Nat
   Program.Equality.
+
 Import ListNotations.
 
 Set Implicit Arguments.
@@ -30,11 +32,23 @@ Inductive sem_op_dfa (S A : Type) (m : dfa S A) : S -> list A -> S -> Prop :=
   | steps     : forall q q' c w,
     sem_op_dfa m (next m q c) w q' ->
     sem_op_dfa m q (c::w) q'.
+  
+Lemma steps_r :
+  forall S A (m : dfa S A) q q' c w,
+    sem_op_dfa m q w  q' ->
+    sem_op_dfa m q (w ++ [c]) (next m q' c).
+Proof.
+  intros.
+  dependent induction H; simpl.
+  - apply one_step.
+  - apply steps, one_step.
+  - apply steps.
+    apply IHsem_op_dfa.
+Qed.
 
-
-Notation "[| m |] w " := (sem_denot_dfa w m) (at level 80).
-Notation "[| m |] ( w , q )" := (fold_left (next m) w q) (at level 80).
-Notation "( m , q1 , w ) --> q2" := (sem_op_dfa m q1 w q2) (at level 80).
+(* Notation "[| m |] w " := (sem_denot_dfa w m) (at level 40).
+Notation "[| m |] ( w , q )" := (fold_left (next m) w q) (at level 40).
+Notation "( m , q1 , w ) --> q2" := (sem_op_dfa m q1 w q2) (at level 40). *)
 
 
 Lemma fold_trans :
@@ -68,7 +82,7 @@ Proof.
   intros. split.
   - intro.
     unfold sem_denot_dfa in H1.
-    exists ([|m|](w, initial_state m)).
+    exists (fold_left (next m) w (initial_state m)).
     split; [assumption | apply H; reflexivity].
   - intros [x [H1 H2]].
     apply fold_trans in H2.
@@ -76,3 +90,157 @@ Proof.
     subst.
     assumption.
 Qed.
+
+Inductive binary := I | O.
+
+Inductive states := S0 | S1 | S2.
+
+Definition m3 : dfa states binary := {|
+  initial_state := S0;
+  is_final s := match s with S0 => true | _ => false end;
+  next s x :=
+    match s, x with
+    | S0, O => S0
+    | S0, I => S1
+    | S1, O => S2
+    | S1, I => S0
+    | S2, O => S1
+    | S2, I => S1
+    end
+|}.
+
+Fixpoint base_2' (w : list binary) : nat :=
+  match w with
+  | [] => 0
+  | I::x => pow 2 (length x) + (base_2' x)
+  | O::x => base_2' x
+  end.
+
+Definition nat_of_bin n :=
+  match n with
+  | I => 1
+  | O => 0
+  end.
+
+Definition base_2 w := fold_left (fun a b => nat_of_bin b + 2 * a) w 0.
+
+Definition divide a b := exists k, b = a*k.
+
+Theorem bin_ind:
+    forall P : list binary -> Prop,
+    P [] ->
+    (forall (w : list binary), P w -> P (w ++ [I])) ->
+    (forall (w : list binary), P w -> P (w ++ [O])) ->
+    forall w, P w.
+Proof.
+Admitted.
+
+Lemma base_2_wI:
+  forall w, 
+  base_2 (w ++ [I]) = 2*(base_2 w) + 1.
+Proof.
+  induction w.
+  - simpl. reflexivity.
+  - unfold base_2.
+    rewrite fold_left_app.
+    simpl.
+    lia.
+Qed.
+
+Lemma base_2_WO:
+  forall w,
+  base_2 (w ++ [O]) = 2 *(base_2 w).
+Proof.
+  induction w.
+  - simpl; reflexivity.
+  - unfold base_2.
+    rewrite fold_left_app.
+    simpl.
+    lia.
+Qed.
+
+Lemma case_S0:
+  forall w,
+  sem_op_dfa m3 S0 w S0 ->
+  divide 3 (base_2 w).
+Proof.
+  intro.
+  elim w using bin_ind.
+  + intro; exists 0; reflexivity.
+  + intros.
+    inversion H0; subst.
+    ++ assert (forall w, [] <> w ++ [I]).
+      * intro. induction w1; discriminate.
+      * apply H1 in H3. contradiction.
+    ++ 
+Abort.
+
+
+(* Lemma trans_S0_I :
+  forall w,
+  sem_op_dfa m3 S0 w S0 ->
+  sem_op_dfa m3 S0 (w ++ [I]) S1.
+Proof.
+  intros.
+  replace (S1) with (next m3 S0 I) by reflexivity.
+  apply steps_r.
+  assumption.
+Qed.
+
+Lemma trans_S0_O :
+  forall w,
+  sem_op_dfa m3 S0 w S0 ->
+  sem_op_dfa m3 S0 (w ++ [O]) S0.
+Proof.
+  intros.
+  replace (S0) with (next m3 S0 O) by reflexivity.
+  apply steps_r.
+  assumption.
+Qed.
+
+Lemma trans_S1_I: 
+  forall w,
+  sem_op_dfa m3 S0 w S1 ->
+  sem_op_dfa m3 S0 (w ++ [I]) S2.
+Proof.
+  intros.
+  replace (S2) with (next m3 S1 I) by reflexivity.
+  apply steps_r.
+  assumption.
+Qed.
+ *)
+
+Lemma sem_app:
+  forall S A (m : dfa S A) q1 q2 q3 w1 w2,
+  sem_op_dfa m q1 w1 q2 ->
+  sem_op_dfa m q2 w2 q3 ->
+  sem_op_dfa m q1 (w1 ++ w2) q3.
+Proof.
+  intros.
+  dependent induction H0.
+  - rewrite app_nil_r. assumption.
+  - apply steps_r. assumption.
+  - dependent induction H.
+    + simpl.
+      apply steps. assumption.
+    + simpl. apply steps.
+      apply steps.
+      assumption.
+    + simpl.
+      apply steps.
+      apply IHsem_op_dfa.
+      ++ assumption.
+      ++ intro.
+
+Qed.
+
+Lemma m3_correct:
+  forall w, 
+  sem_op_dfa m3 S0 w S0 ->
+  divide 3 (base_2 w).
+Proof.
+  intro.
+  elim w using bin_ind.
+  + intro.
+    exists 0; reflexivity.
+  + intros.
